GradVer19Theorems.v
@@ -1,0 +1,100 @@
+Load GradVer18LemmaHI.
+Import Semantics.
+
+
+Lemma dynSemStarNotModifies : forall x ss H1 H2 r1 r2 A1 A2,
+  (∀ s', In s' ss → ¬ writesTo x s') ->
+  dynSemStar
+    (H1, [(r1, A1, ss)])
+    (H2, [(r2, A2, [])]) ->
+  r1 x = r2 x.
+Proof.
+  induction ss; intros; simpl in *.
+  - inversionx H3; try tauto.
+    inversionx H4.
+  - inversionx H3.
+    rename H4 into ds.
+    rename H5 into dss.
+    assert (¬ writesTo x0 a) as wt1. apply H0. tauto.
+    assert (∀ s' : s, In s' ss → ¬ writesTo x0 s') as wt2. intros. apply H0. tauto.
+    inversionx ds; simpl in wt1.
+    * apply IHss in dss; auto.
+    * apply IHss in dss; auto.
+      unfold rhoSubst in dss.
+      dec (x_dec x0 x1); try tauto.
+      contradict wt1.
+      constructor.
+    * apply IHss in dss; auto.
+      unfold rhoSubst in dss.
+      dec (x_dec x0 x1); try tauto.
+      contradict wt1.
+      constructor.
+    * apply IHss in dss; auto.
+      unfold rhoSubst in dss.
+      dec (x_dec x0 xresult); try tauto.
+      contradict wt1.
+      constructor.
+    * admit.
+    * apply IHss in dss; auto.
+    * apply IHss in dss; auto.
+    * apply IHss in dss; auto.
+      unfold rhoSubst in dss.
+      dec (x_dec x0 x1); try tauto.
+      contradict wt1.
+      constructor.
+Admitted.
+
+
+
+Lemma dynSemStarNotModifiesH : forall ss H1 H2 r1 r2 A1 A2 A v,
+  ~ In A A1 ->
+  dynSemStar
+    (H1, [(r1, A1, ss)])
+    (H2, [(r2, A2, [])]) ->
+  evalA'_d H1 A = Some v ->
+  evalA'_d H2 A = Some v.
+Proof.
+  induction ss; intros; simpl in *.
+  - inversionx H3; try tauto.
+    inversionx H5.
+  - inversionx H3.
+    rename H5 into ds.
+    rename H6 into dss.
+    inversionx ds.
+    * eapply IHss in dss; eauto.
+      destruct A. unfold evalA'_d in *. simpl in *.
+      unfold HSubst.
+      dec (o_dec o1 o0); try tauto.
+      destruct (H1 o0); try discriminate.
+      destruct p0. simpl in *.
+      dec (string_dec f1 f0); try tauto.
+    * eapply IHss in dss; eauto.
+    * eapply IHss in dss; eauto.
+      + unfold not. intros.
+        apply in_app_iff in H3.
+        intuition.
+        apply in_map_iff in H5.
+        unf. subst.
+        unfold evalA'_d, HeapNotSetAt in *.
+        simpl in *.
+        rewrite H12 in *.
+        discriminate.
+      + unfold Halloc.
+        rewrite H13.
+        destruct A. unfold evalA'_d in *. simpl in *.
+        dec (o_dec o0 o1); try tauto.
+        unfold HeapNotSetAt in H12. rewrite H12 in *.
+        discriminate.
+    * eapply IHss in dss; eauto.
+    * admit.
+    * eapply IHss in dss; eauto.
+    * eapply IHss in dss; eauto.
+      unfold not in *. intros. contradict H0.
+      apply InAexcept in H3.
+      assumption.
+    * eapply IHss in dss; eauto.
+Admitted.
+
+
+
+
